implemented DFS in Coq.
We designed the algorithm by tail-recursion and passing a context to
explicitly hold the stack. Here, stack is a list of frame; each frame
carries a node and its succesors to visit.

At each recursion, we find the next unvisited successor v of the last
node on
stack, and then do recursion by adding v into visited nodes. Therefore,
the size of visited nodes also increase at each recursion, which
simplifies
termination proofs.

On performance, the extracted DFS is slightly slower than the one we
implemented in OCaml. This could be caused by at least two issues
  1) Coq DFS takes a graph and an additional context at each call, OCaml
     DFS only needs the graph. The size of the addition context is as
     large as the graph.
  2) The extraction from "Program Fixpoint" has additional curry and
     uncurry at each recursion, since its internal representation is a
     function with only one argument.



git-svn-id: https://webdav.seas.upenn.edu/svn/sol/vol@3991 eef5ea85-cc2e-0410-bd84-0fae1f012da8

src3.0/Vellvm/Dominators/fast_iter.v
@@ -1,25 +1,498 @@
 Require Export Coqlib.
 Require Export Iteration.
 Require Export Maps.
+Require Import syntax.
+Require Import Kildall.
+Require Import infrastructure_props.
+Require Import Metatheory.
 
+Import LLVMsyntax.
 
-(*
-Program Fixpoint DFS (succs:ATree.t ls) (visited:ATree.t ls)
-  (acc:ATree.t positive * PTree.t l) 
-  (po:positive) (todo:ls) 
-  {measure ((fun s' v' => f s' - length) visited succs)} :
-  (ATree.t positive * PTree.t l) := 
-match todo with
-| nil => acc
-| next::todo' =>
-    match ATree.get next visited with
-    | None => 
-        let acc' := DFS succs visited acc po (succs!!!next) in
-        acc'
-    | Some _ => DFS succs visited acc po todo'
+Section MoreMove. (* copied from dtree.v *)
+
+Variable A: Type.
+Hypothesis Hdec: forall x y : A, {x = y} + {x <> y}.
+
+Lemma remove_length: forall (a: A) (l1: list A),
+  (length (List.remove Hdec a l1) <= length l1)%nat.
+Proof.
+  induction l1; simpl; intros.
+    omega.
+    destruct (Hdec a a0); subst; simpl; omega.
+Qed.
+
+Lemma remove_in_length: forall (a: A) (l1: list A),
+  In a l1 -> (length (List.remove Hdec a l1) < length l1)%nat.
+Proof.
+  induction l1; simpl; intros.
+    inv H.
+
+    destruct H as [H | H]; subst.
+      destruct (Hdec a a); try congruence.
+      assert (J:=@remove_length a l1). omega.
+
+      destruct (Hdec a a0); subst.
+        assert (J:=@remove_length a0 l1). omega.
+        assert (J:=@IHl1 H). simpl. omega.
+Qed.
+
+Lemma remove_neq_in: forall (a b:A) (l1: list A),
+  a <> b ->
+  In a l1 ->
+  In a (List.remove Hdec b l1).
+Proof.
+  induction l1; simpl; intros; auto.
+    destruct H0 as [H0 | H0]; subst.
+      destruct (Hdec b a); subst; simpl; auto.
+        congruence.
+      destruct (Hdec b a0); subst; simpl; auto.
+Qed.
+
+Lemma remove_notin_incl: forall (a : A) (l2 l1 : list A)
+  (Hinc : incl l1 l2) (Hnotin : ~ In a l1),
+  incl l1 (List.remove Hdec a l2).
+Proof.
+  intros. intros x Hin.
+  destruct (Hdec x a); subst.
+    congruence.
+    apply remove_neq_in; auto.
+Qed.
+
+Lemma remove_neq_in': forall (a b:A) (l1: list A),
+  In a (List.remove Hdec b l1) ->
+  In a l1 /\ a <> b.
+Proof.
+  induction l1; simpl; intros; auto.
+    destruct (Hdec b a0); subst; simpl.
+      apply IHl1 in H.
+      destruct H as [H1 H2].
+      split; auto.
+
+      simpl in H.
+      destruct H as [H | H]; subst; auto.
+      apply IHl1 in H.
+      destruct H as [H1 H2].
+      split; auto.
+Qed.
+
+End MoreMove.
+
+Record Frame := mkFrame {
+  Fr_name: l;
+  Fr_scs: ls
+}.
+
+Fixpoint find_next_visit_in_scs (visited: ATree.t unit) (scs: ls) 
+  : option (l * ls) :=
+match scs with
+| nil => None
+| sc::scs' => 
+    match ATree.get sc visited with
+    | None => Some (sc, scs')
+    | _ => find_next_visit_in_scs visited scs'
     end
 end.
-*)
+
+Record PostOrder := mkPO {
+  PO_cnt: positive;
+  PO_a2p: ATree.t positive
+}.
+
+Definition postorder_inc (po:PostOrder) (v:l) : PostOrder :=
+let '(mkPO cnt a2p) := po in
+mkPO (Psucc cnt) (ATree.set v cnt a2p).
+
+Fixpoint find_next_visit_in_stk (succs: ATree.t ls)
+  (visited: ATree.t unit) (po:PostOrder) (frs: list Frame) 
+  : l * list Frame * PostOrder + PostOrder :=
+match frs with
+| nil => inr po
+| mkFrame v scs::frs' => 
+    match find_next_visit_in_scs visited scs with
+    | Some (sc, scs') => 
+        inl (sc, mkFrame sc (succs!!!sc)::mkFrame v scs'::frs', po)
+    | None => find_next_visit_in_stk succs visited (postorder_inc po v) frs'
+    end
+end.
+
+Definition children_of_tree A (tree: ATree.t (list A)) :=
+  flat_map snd (ATree.elements tree).
+
+Definition parents_of_tree A (tree: ATree.t A) :=
+  List.map fst (ATree.elements tree).
+
+Implicit Arguments children_of_tree [A].
+Implicit Arguments parents_of_tree [A].
+
+Require Import Program.Tactics.
+
+Ltac inv_mbind_app :=
+  match goal with
+  | H: _ = match ?e with
+       | Some _ => _
+       | None => _
+       end |- _ => remember e as R; destruct R
+  | H: match ?e with
+       | Some _ => _
+       | None => _
+       end = _ |- _ => remember e as R; destruct R
+  end.
+
+Lemma find_next_visit_in_scs_spec: forall visited scs sc scs'
+  (Hfind : Some (sc, scs') = find_next_visit_in_scs visited scs),
+  incl (sc::scs') scs /\ ATree.get sc visited = None.
+Proof.
+  induction scs as [|sc scs]; simpl; intros.
+    congruence.
+
+    inv_mbind_app.
+      apply IHscs in Hfind.
+      destruct_pairs.
+      split; eauto with datatypes v62.
+    
+      uniq_result.
+      split; eauto with datatypes v62.
+Qed.
+
+Lemma successors_list_spec: forall a scss l0,
+  In a (scss!!!l0) -> exists scs, scss!l0 = Some scs /\ In a scs.
+Proof.
+  unfold successors_list.
+  intros.
+  destruct (scss!l0); [eauto | tauto].
+Qed.
+
+Lemma children_in_children_of_tree: forall succs l0,
+  incl succs !!! l0 (children_of_tree succs).
+Proof.
+  intros.
+  intros x Hin.
+  apply in_flat_map.
+  apply successors_list_spec in Hin.
+  destruct_conjs.
+  eauto using ATree.elements_correct.
+Qed.
+
+Lemma incl__length_le: forall A (eq_dec : forall x y : A, {x = y}+{x <> y})
+  (l1:list A) (Huniq: list_norepet l1) (l2:list A) (Hinc: incl l1 l2), 
+  (length l1 <= length l2)%nat.
+Proof.
+  induction 2 as [|hd tl Hnotin Huniq IH]; simpl; intros.
+    auto with datatypes v62.
+
+    assert (incl tl (List.remove eq_dec hd l2)) as Hinc'.
+      apply remove_notin_incl; eauto with datatypes v62.
+    apply IH in Hinc'.
+    assert (length (List.remove eq_dec hd l2) < length l2)%nat as Hle.
+      apply remove_in_length; auto with datatypes v62.
+    omega.
+Qed.
+
+Lemma length_le__length_lt: forall A 
+  (eq_dec : forall x y : A, {x = y}+{x <> y})
+  (a:A) (l2:list A) (l1:list A) 
+  (Huniq: list_norepet l1) (Hinc: incl l1 l2)  
+  (Hnotin: ~ In a l1) (Hin: In a l2), 
+  (length l1 < length l2)%nat.
+Proof.
+  intros.
+  assert (incl l1 (List.remove eq_dec a l2)) as Hinc'.
+    apply remove_notin_incl; eauto with datatypes v62.
+  apply incl__length_le in Hinc'; auto.
+  assert (length (List.remove eq_dec a l2) < length l2)%nat as Hle.
+    apply remove_in_length; auto with datatypes v62.
+  omega.
+Qed.
+
+Lemma parents_of_tree_spec: forall A l0 (tr: ATree.t A),
+  In l0 (parents_of_tree tr) <-> exists a, In (l0, a) (ATree.elements tr).
+Proof.
+  unfold parents_of_tree.
+  intros.
+  split; intro J.
+    apply in_map_iff in J.
+    destruct J as [[x1 x2] [J1 J2]]. subst. eauto.
+
+    apply in_map_iff.
+    destruct J as [y J]. exists (l0, y). auto.
+Qed.
+
+Lemma notin_tree__notin_parents_of_tree: forall (visited : ATree.t unit)
+  (l0 : l) (H0 : visited ! l0 = None),
+  ~ In l0 (parents_of_tree visited).
+Proof.
+  intros.
+  intros Hin'. apply parents_of_tree_spec in Hin'.
+  destruct Hin' as [a Hin'].
+  apply ATree.elements_complete in Hin'. 
+  congruence.
+Qed.
+
+Lemma in_tree__in_parents_of_tree: forall (visited : ATree.t unit) a
+  (l0 : l) (H0 : visited ! l0 = Some a),
+  In l0 (parents_of_tree visited).
+Proof.
+  intros.
+  apply parents_of_tree_spec. 
+  apply ATree.elements_correct in H0.  eauto.
+Qed.
+
+Lemma parents_children_of_tree__inc__length_le: forall A (visited:ATree.t A)
+  succs (Hinc: incl (parents_of_tree visited) (children_of_tree succs)),
+  (length (parents_of_tree visited) <= length (children_of_tree succs))%nat.
+Proof.
+  intros. 
+  apply incl__length_le; auto.
+    apply ATree.elements_keys_norepet.
+Qed.
+
+Lemma list_equiv_nil: forall A (l1:list A) (Heq: list_equiv nil l1), l1 = nil.
+Proof.
+  intros.
+  destruct l1 as [|x l1]; auto.
+  destruct (Heq x) as [_ J1].
+  assert (In x (x::l1)) as J. auto with datatypes v62.
+  apply J1 in J. tauto.
+Qed.
+
+Lemma norepet_equiv__length_eq: forall A (l1:list A)
+  (Huniq1: list_norepet l1) (l2:list A) (Huniq2: list_norepet l2)
+  (Heq: list_equiv l1 l2),
+  (length l1 = length l2)%nat.
+Proof.
+  induction 1; simpl; intros.
+    apply list_equiv_nil in Heq. subst. auto.
+
+    destruct (Heq hd) as [J1 _].
+    assert (In hd (hd::tl)) as J2. auto with datatypes v62.
+    apply J1 in J2.
+    apply in_split in J2.
+    destruct_conjs; subst.
+    rewrite app_length. simpl.
+    rewrite IHHuniq1 with (l2:=J2++H0).
+      rewrite app_length.
+      omega.
+
+      apply list_norepet_append_commut in Huniq2.
+      simpl_env in Huniq2.
+      apply list_norepet_append_commut.
+      apply list_norepet_app in Huniq2.
+      tauto.
+
+      apply list_norepet_append_commut in Huniq2.
+      simpl_env in Huniq2.
+      apply list_norepet_app in Huniq2.
+      destruct_conjs.
+      intro x.
+      destruct (Heq x) as [J1' J2'].
+      split; intro J.
+        assert (Hin: In x (hd::tl)). auto with datatypes v62.
+        apply J1' in Hin.
+        destruct_in Hin; auto with datatypes v62.
+        destruct_in Hin; auto with datatypes v62.
+
+        assert (Hin: In x (J2 ++ hd :: H0)). 
+          destruct_in J; auto with datatypes v62.
+        apply J2' in Hin.
+        destruct_in Hin; auto with datatypes v62.
+        assert (x <> x) as Hf.
+          apply H3; simpl; auto with datatypes v62.     
+          destruct_in J; auto with datatypes v62.
+        congruence.
+Qed.
+
+Lemma norepet_equiv__length_cons_eq: forall A l1 l2 (a:A)
+  (Huniq1: list_norepet l1) (Huniq2: list_norepet l2)
+  (Hnotin: ~ In a l1) (Heq: list_equiv l2 (a::l1)),
+  (length l2 = length l1 + 1)%nat.
+Proof.
+  intros.
+  apply norepet_equiv__length_eq in Heq; auto.
+    simpl in *. omega.
+    constructor; auto.
+Qed.
+
+Lemma parents_of_tree_succ_len: forall (visited : ATree.t unit)
+  (l0 : l) (H0 : visited ! l0 = None),
+  length (parents_of_tree (ATree.set l0 tt visited)) =
+    (length (parents_of_tree visited) + 1)%nat.
+Proof.
+  intros.
+  unfold parents_of_tree.
+  apply norepet_equiv__length_cons_eq with (a:=l0); 
+    auto using ATree.elements_keys_norepet.
+    apply notin_tree__notin_parents_of_tree; auto.
+
+    intro x; split; intro Hin.
+      apply parents_of_tree_spec in Hin.
+      destruct_conjs.
+      apply ATree.elements_complete in H. 
+      rewrite ATree.gsspec in H.
+      destruct_if.
+        auto with datatypes v62.
+
+        apply in_tree__in_parents_of_tree in H2.
+        auto with datatypes v62.
+
+      apply parents_of_tree_spec.
+      destruct_in Hin.
+        exists tt.
+        apply ATree.elements_correct.
+        rewrite ATree.gsspec.
+        destruct_if. 
+          congruence.
+
+        apply parents_of_tree_spec in Hin.
+        destruct_conjs.
+        exists Hin. 
+        apply ATree.elements_correct.
+        rewrite ATree.gsspec.
+        destruct_if. 
+          apply ATree.elements_complete in H.  
+          congruence.
+
+          apply ATree.elements_complete in H. auto.
+Qed.
+
+Lemma find_next_visit_in_stk_spec1: forall succs visited (stk : list Frame)
+  (Hp : Forall (fun fr : Frame => 
+                incl (Fr_scs fr) (children_of_tree succs)) stk)  
+  po (next : l) (stk' : list Frame) po'
+  (Hfind : inl (next, stk', po') = find_next_visit_in_stk succs visited po stk),
+  Forall (fun fr : Frame => incl (Fr_scs fr) (children_of_tree succs)) stk'.
+Proof.
+  induction 1 as [|[v scs]]; simpl; intros.
+    congruence.
+        
+    inv_mbind_app; eauto 2.
+      destruct_let.
+      uniq_result.
+      apply find_next_visit_in_scs_spec in HeqR.
+      destruct_pairs.
+      constructor.
+        simpl. apply children_in_children_of_tree.
+        constructor; auto.
+          simpl in *.
+          eauto with datatypes v62.
+Qed.
+
+Lemma find_next_visit_in_stk_spec3_helper: forall 
+  (succs : ATree.t (list MetatheoryAtom.AtomImpl.atom))
+  (visited : ATree.t unit)
+  (Hinc : incl (parents_of_tree visited) (children_of_tree succs))
+  (v : l) (scs : ls)
+  (H : incl (Fr_scs {| Fr_name := v; Fr_scs := scs |})
+        (children_of_tree succs))
+  (l0 : l) (l1 : ls) (H0 : incl (l0 :: l1) scs)
+  (H1 : visited ! l0 = None),
+  (length (parents_of_tree visited) < length (children_of_tree succs))%nat.
+Proof.
+  intros.
+  assert (In l0 (children_of_tree succs)) as Hin.
+    apply H. simpl. apply H0. xsolve_in_list.
+  eapply length_le__length_lt; eauto.
+    apply ATree.elements_keys_norepet; auto.
+    apply notin_tree__notin_parents_of_tree; auto.
+Qed.
+
+Lemma find_next_visit_in_stk_spec3: forall succs visited 
+  (Hinc: incl (parents_of_tree visited) (children_of_tree succs))
+  (stk : list Frame) 
+  (Hp : Forall (fun fr : Frame => 
+                incl (Fr_scs fr) (children_of_tree succs)) stk)
+  (next : l) (stk' : list Frame) po po'
+  (Hfind : inl (next, stk', po') =
+                   find_next_visit_in_stk succs visited po stk),
+  (length (children_of_tree succs) -
+    length (parents_of_tree (ATree.set next tt visited)) <
+    length (children_of_tree succs) - length (parents_of_tree visited))%nat.
+Proof.
+  induction 2 as [|[v scs]]; simpl; intros.
+    congruence.
+
+    inv_mbind_app; eauto 2.
+      destruct_let.
+      uniq_result.
+      apply find_next_visit_in_scs_spec in HeqR.
+      destruct_pairs.
+      assert (length (parents_of_tree (ATree.set l1 tt visited)) =
+                length (parents_of_tree visited) + 1)%nat as Heq.
+        apply parents_of_tree_succ_len; auto.
+      assert (length (parents_of_tree visited) <
+                length (children_of_tree succs))%nat as Hlt.
+        eapply find_next_visit_in_stk_spec3_helper; eauto.
+      omega.
+Qed.
+
+Lemma find_next_visit_in_stk_spec2: forall (succs : ATree.t ls) 
+  (visited : ATree.t unit)
+  (Hinc : incl (parents_of_tree visited) (children_of_tree succs))
+  (stk : list Frame)
+  (Hp : Forall (fun fr : Frame => 
+                incl (Fr_scs fr) (children_of_tree succs)) stk)
+  (next : l) (stk' : list Frame) po po'
+  (Hfind : inl (next, stk', po') = find_next_visit_in_stk succs visited po stk),
+  incl (parents_of_tree (ATree.set next tt visited))
+    (children_of_tree succs).
+Proof.
+  induction 2 as [|[v scs] ? IH]; simpl; intros.
+    congruence.
+
+    inv_mbind_app; eauto 2.
+      destruct_let.
+      uniq_result.
+      apply find_next_visit_in_scs_spec in HeqR.
+      destruct_pairs.
+      intros x Hin.
+      apply parents_of_tree_spec in Hin.
+      destruct Hin as [? Hin].
+      apply ATree.elements_complete in Hin. 
+      rewrite ATree.gsspec in Hin.
+      destruct_if.
+        eauto with datatypes v62.
+           
+        apply ATree.elements_correct in H2. 
+        apply Hinc.
+        apply List.in_map with (f:=fst) in H2; auto.
+Qed.
+
+Program Fixpoint dfs_aux (succs: ATree.t ls)
+  (visited: ATree.t unit) (po:PostOrder) (stk: list Frame) 
+  (Hp: List.Forall 
+         (fun fr => incl (Fr_scs fr) (children_of_tree succs)) stk /\
+       incl (parents_of_tree visited) (children_of_tree succs))
+  {measure 
+    ((fun succs acc => 
+      (length (children_of_tree succs) - 
+       length (parents_of_tree visited))%nat) succs visited) }
+  : PostOrder :=
+  match find_next_visit_in_stk succs visited po stk with
+  | inr po' => po'
+  | inl (next, stk', po') => dfs_aux succs (ATree.set next tt visited) po' stk' _
+  end.
+Next Obligation.
+  split.
+    eapply find_next_visit_in_stk_spec1; eauto.
+    eapply find_next_visit_in_stk_spec2; eauto.
+Qed.
+Next Obligation.
+  eapply find_next_visit_in_stk_spec3; eauto.
+Qed.
+
+Lemma parents_of_empty_tree: forall A,
+  parents_of_tree (ATree.empty A) = nil.
+Proof. auto. Qed.
+
+Program Definition dfs (succs: ATree.t ls) (entry:l) (pinit:positive) : PostOrder :=
+dfs_aux succs (ATree.empty unit) (mkPO pinit (ATree.empty positive)) 
+  (mkFrame entry (succs!!!entry)::nil) _.
+Next Obligation.
+  split.  
+    constructor; auto.
+      apply children_in_children_of_tree.
+    rewrite parents_of_empty_tree. 
+    intros x Hin. tauto.
+Qed.
 
 Notation "a ! b" := (PTree.get b a) (at level 1).
 Notation "a !! b" := (PMap.get b a) (at level 1).
@@ -637,11 +1110,6 @@ End Kildall.
 
 End Weak_Dataflow_Solver.
 
-Require Import syntax.
-Require Import infrastructure.
-Import LLVMsyntax.
-Parameter dfs : ATree.t ls -> l -> positive -> ATree.t positive * PTree.t l.
-
 Fixpoint asucc_psucc_aux (mapping: ATree.t positive)  
                          (pred: PTree.t (list positive))
                          (pfrom: positive) (tolist: list l)
@@ -708,12 +1176,13 @@ match input with
 end.
 
 Require analysis.
+Require Import infrastructure.
 
 Definition dom_analyze (f: fdef) : PMap.t LDoms.t :=
   let asuccs := analysis.successors f in
   match LLVMinfra.getEntryBlock f with
   | Some (block_intro le _ _ _) =>
-      let '(a2p, p2a) := dfs asuccs le 1%positive in
+      let 'mkPO _ a2p := dfs asuccs le 1%positive in
       let psuccs := asuccs_psuccs a2p asuccs in
       match ATree.get le a2p with
       | Some pe => 
